Phi_Semantics/PhSem_MoV.thy
@@ -522,4 +522,191 @@ end
 end
 
 
+
+locale MoV_res =
+  MoV Rep_of_Val +
+  partial_map_resource Res \<open>\<lambda>blk. discrete ` Rep_of_Val ` Well_Type (typ_of_blk blk)\<close>
+  for Res :: "('blk \<Rightarrow> 'Rep discrete option) resource_entry"
+  and Rep_of_Val :: \<open>VAL \<Rightarrow> 'Rep\<close>
+  and typ_of_blk :: \<open>'blk \<Rightarrow> TY\<close>
+
+locale perm_MoV_fiction =
+  MoV Rep_of_Val +
+  pointwise_base_fiction_for_partial_mapping_resource
+      Res \<open>\<lambda>blk. \<F>_functional (Rep_of_Val_ins (typ_of_blk blk)) (Rep_of_Val_ins_dom (typ_of_blk blk)) \<Zcomp>
+                 \<F>_functional ((\<circ>) to_share \<circ> Map_of_Val_ins) (Map_of_Val_ins_dom (typ_of_blk blk))\<close>
+      Fic \<open>\<lambda>blk. discrete ` Rep_of_Val ` Well_Type (typ_of_blk blk)\<close>
+  for Res :: "('blk \<Rightarrow> 'Rep discrete option) resource_entry"
+  and Rep_of_Val :: \<open>VAL \<Rightarrow> 'Rep\<close>
+  and typ_of_blk :: \<open>'blk \<Rightarrow> TY\<close>
+  and null_blk :: 'blk
+  and Fic :: "('blk \<Rightarrow> aggregate_path \<Rightarrow> VAL discrete share option) fiction_entry"
+begin
+
+sublocale MoV_res Res Rep_of_Val typ_of_blk ..
+
+lemma getter_rule:
+  \<open> valid_index (typ_of_blk blk) idx
+\<Longrightarrow> \<p>\<r>\<e>\<m>\<i>\<s>\<e> u_idx \<in> Well_Type (index_type idx (typ_of_blk blk)) \<and> cblk = blk
+\<Longrightarrow> \<p>\<r>\<e>\<m>\<i>\<s>\<e> 0 < n
+\<Longrightarrow> \<p>\<r>\<o>\<c> R.\<phi>R_get_res_entry' cblk \<lbrace> 1(blk := n \<odivr> (to_share \<circ> idx \<tribullet>\<^sub>m (map_option discrete \<circ> Map_of_Val u_idx))) \<Ztypecolon> \<phi> Itself \<longmapsto>
+      \<lambda>ret. 1(blk := n \<odivr> (to_share \<circ> idx \<tribullet>\<^sub>m (map_option discrete \<circ> Map_of_Val u_idx))) \<Ztypecolon> \<phi> Itself
+          \<s>\<u>\<b>\<j> x. ret = \<phi>arg (discrete (Rep_of_Val x)) \<and> x \<in> Well_Type (typ_of_blk blk) \<and> index_value idx x = u_idx \<rbrace>\<close>
+  unfolding Premise_def
+  subgoal premises prems proof -
+
+  have [simp]: \<open>cblk = blk\<close>
+    by (simp add: prems(2))
+
+  have simp1: \<open>
+      (A x \<s>\<u>\<b>\<j> x. B x \<and> x \<in> Rep_of_TY (typ_of_blk blk) \<and> x \<in> Rep_of_Val ` {a. index_value idx a = u_idx \<and> a \<in> Well_Type (typ_of_blk cblk)})
+    = (A (Rep_of_Val v) \<s>\<u>\<b>\<j> v. B (Rep_of_Val v) \<and> v \<in> Well_Type (typ_of_blk blk) \<and> index_value idx v = u_idx) \<close>
+  for A B C ret TY S
+  unfolding BI_eq_iff split_discrete_ex
+  by (auto simp: image_iff Bex_def)
+
+  show ?thesis
+    by (rule "_getter_rule_2_"[OF _ fiction_Map_of_Val_ins_perm_projection_half_BYTE,
+              where k=cblk and k'=blk and idx1=idx and u_idx1=u_idx,
+              simplified split_discrete_ExBI inj_image_mem_iff inj_discrete simp1],
+        insert prems, simp+)
+qed .
+
+
+context notes mul_carrier_option_def[simp] option.pred_True[simp] begin
+
+lemma allocate_rule:
+  \<open> \<p>\<r>\<e>\<m>\<i>\<s>\<e> (\<forall>r. finite (dom r) \<longrightarrow> (\<exists>blk. blk \<notin> dom r \<and> typ_of_blk blk = TY \<and> blk \<noteq> null_blk))
+\<Longrightarrow> \<p>\<r>\<e>\<m>\<i>\<s>\<e> (\<forall>v\<in>U. v \<in> Well_Type TY)
+\<Longrightarrow> \<p>\<r>\<o>\<c> R.\<phi>R_allocate_res_entry (\<lambda>blk. typ_of_blk blk = TY \<and> blk \<noteq> null_blk) (\<lambda>k. {Some (discrete (Rep_of_Val v)) |v. v\<in>U })
+      \<lbrace> Void \<longmapsto> \<lambda>ret. 1(blk := to_share \<circ> (map_option discrete \<circ> Map_of_Val v)) \<Ztypecolon> \<phi> Itself
+                  \<s>\<u>\<b>\<j> blk v. ret = \<phi>arg blk \<and> v \<in> U \<and> typ_of_blk blk = TY \<and> blk \<noteq> null_blk  \<rbrace> \<close>
+  unfolding Premise_def
+  subgoal premises prems proof-
+
+  note pointwise_set_UNIV[simp] \<F>_functional_condition_Map_of_Val_ins_dom[simp]
+
+  have t1[simp]: \<open>v \<in> U \<Longrightarrow> Val_of_Rep TY (Rep_of_Val v) = v\<close> for v
+    using prems(2) by auto
+  have [simp]:
+       \<open>{(1, to_share \<circ> (map_option discrete \<circ> Map_of_Val (Val_of_Rep TY (Rep_of_Val v)))) |v. v \<in> U}
+      = {(1, to_share \<circ> (map_option discrete \<circ> Map_of_Val v)) |v. v \<in> U}\<close>
+    by force
+
+  note rule = sep_refinement_stepwise[
+        OF refinement_frame[OF Rep_of_Val_ins.\<F>_functional_refinement'[simplified]]
+           sep_refinement_stepwise[
+                    OF refinement_frame[OF Map_of_Val_ins.\<F>_functional_refinement'[simplified]]
+                       pointwise_to_share.\<F>_functional_refinement'[where B=\<open>Map_of_Val_ins ` B\<close> for B, unfolded defined_set_in_image]
+                       pointwise_to_share.\<F>_functional_projection,
+                    where B6=\<open>Rep_of_Val_ins TY ` B\<close> for B, unfolded defined_set_in_image],
+        where a35=\<open>None\<close> and B22=\<open>{Some (discrete (Rep_of_Val v)) |v. v \<in> U}\<close>,
+        simplified,
+        OF _ _ _ refinement_projections_stepwise_UNIV_paired[
+            OF Map_of_Val_ins.\<F>_functional_projection
+               pointwise_to_share.\<F>_functional_projection,
+            where Dc=\<open>{1}\<close>,
+            simplified]]
+
+  show ?thesis
+    by (rule "__allocate_rule_3__"[
+          where U =\<open>\<lambda>k. {Some (discrete (Rep_of_Val v)) |v. v\<in>U }\<close>
+            and U'=\<open>\<lambda>k. {to_share \<circ> (map_option discrete \<circ> Map_of_Val v) |v. v \<in> U}\<close> , simplified],
+        unfold \<F>_functional_comp[where f=\<open>(\<circ>) to_share\<close> and Df=\<open>UNIV\<close>, simplified, simp]
+               one_option_def,
+        simp, rule rule,
+        simp add: subset_iff, insert Rep_of_Val_ins_dom_eval(2) prems(2), blast,
+        simp add: \<F>_functional_condition_Rep_of_Val_ins_dom,
+        simp add: subset_iff, force,
+        simp add: R.in_invariant inj_image_mem_iff, force,
+        clarsimp simp add: R.in_invariant Ball_def dom1_dom, metis dom_map_option_comp prems(1))
+qed .
+
+lemma setter_rule:
+  assumes EQ: \<open>\<p>\<r>\<e>\<m>\<i>\<s>\<e> cblk = blk\<close>
+  shows \<open> valid_index (typ_of_blk blk) idx
+      \<Longrightarrow> \<p>\<r>\<e>\<m>\<i>\<s>\<e> v \<in> Well_Type (index_type idx (typ_of_blk blk))
+      \<Longrightarrow> \<p>\<r>\<e>\<m>\<i>\<s>\<e> u_idx \<in> Well_Type (index_type idx (typ_of_blk blk))
+      \<Longrightarrow> \<p>\<r>\<e>\<m>\<i>\<s>\<e> (\<forall>x\<in>Well_Type (typ_of_blk blk). index_mod_value cidx (\<lambda>_. v) x = index_mod_value idx (\<lambda>_. v) x)
+      \<Longrightarrow> \<p>\<r>\<o>\<c> R.\<phi>R_set_res (map_fun_atS cblk (\<lambda>h. {Some (map_discrete (map_Rep (typ_of_blk cblk) (index_mod_value cidx (\<lambda>_. v))) (the h))}))
+            \<lbrace> 1(blk := to_share \<circ> idx \<tribullet>\<^sub>m (map_option discrete \<circ> Map_of_Val u_idx)) \<Ztypecolon> \<phi> Itself \<longmapsto>
+              \<lambda>\<r>\<e>\<t>. 1(blk := to_share \<circ> idx \<tribullet>\<^sub>m (map_option discrete \<circ> Map_of_Val v)) \<Ztypecolon> \<phi> Itself \<rbrace> \<close>
+  unfolding Premise_def
+  by (simp add: EQ[unfolded Premise_def],
+      rule "_setter_rule_2_"[where f=\<open>\<lambda>h. {Some (map_discrete (map_Rep (typ_of_blk blk) (index_mod_value cidx (\<lambda>_. v))) h)}\<close>
+                        and V=\<open>discrete ` Rep_of_Val ` {a. index_value idx a = u_idx \<and> a \<in> Well_Type (typ_of_blk blk)}\<close>
+                        and F=\<open>\<lambda>_. {to_share o idx \<tribullet>\<^sub>m (map_option discrete \<circ> Map_of_Val v)}\<close>
+                        for idx cidx v u_idx,
+                      simplified,
+                      OF _ fiction_Map_of_Val_perm_partial_refinement_BYTE[simplified]
+                           fiction_Map_of_Val_ins_perm_projection_BYTE[simplified]],
+      simp,
+      assumption,
+      assumption,
+      assumption,
+      assumption,
+      assumption,
+      assumption,
+      clarsimp simp add: split_discrete_meta_all inj_image_mem_iff index_mod_value_welltyp image_iff Bex_def,
+      metis Val_of_Rep_inj index_mod_value_welltyp map_Rep_def)
+
+lemma deallocate_rule:
+  \<open> \<p>\<r>\<e>\<m>\<i>\<s>\<e> v \<in> Well_Type (typ_of_blk blk)
+\<Longrightarrow> \<p>\<r>\<o>\<c> R.\<phi>R_set_res (map_fun_atS blk (\<lambda>_. {None}))
+      \<lbrace> 1(blk := to_share \<circ> (map_option discrete \<circ> Map_of_Val v)) \<Ztypecolon> \<phi> Itself \<longmapsto>
+        \<lambda>\<r>\<e>\<t>. 1 \<Ztypecolon> \<phi> Itself \<rbrace> \<close>
+  unfolding Premise_def
+subgoal premises prems
+proof -
+  have [simp]:
+    \<open>Map.empty \<circ> the = Map.empty\<close>
+    unfolding fun_eq_iff by simp
+
+  note inj_image_mem_iff[simp] pointwise_set_UNIV[simp] \<F>_functional_condition_Map_of_Val_ins_dom[simp]
+       \<F>_functional_comp[where f=\<open>(\<circ>) to_share\<close> and Df=\<open>UNIV\<close>, simplified, symmetric, simp]
+
+  have [simp]: \<open>Val_of_Rep (typ_of_blk blk) (Rep_of_Val v) = v\<close>
+    by (simp add: prems)
+
+  note rule1 = refinement_projections_stepwise_UNIV_paired[
+          OF Map_of_Val_ins.\<F>_functional_projection
+             pointwise_to_share.\<F>_functional_projection,
+          where Dc=\<open>{Some (discrete v)}\<close>,
+          simplified]
+
+  show ?thesis
+apply simp
+apply (rule "_setter_rule_2_"[where f=\<open>\<lambda>_. {None}\<close> and V=\<open>{discrete v}\<close> and F=\<open>\<lambda>_. 1\<close> for v, simplified])
+apply (simp,
+        unfold refinement_source_subjection, rule impI,
+        rule sep_refinement_stepwise [
+            OF refinement_frame[OF Rep_of_Val_ins.\<F>_functional_refinement[simplified]]
+               sep_refinement_stepwise[
+                        OF refinement_frame[OF Map_of_Val_ins.\<F>_functional_refinement[simplified]]
+                           pointwise_to_share.\<F>_functional_refinement
+                           pointwise_to_share.\<F>_functional_projection],
+            where a16=\<open>Some (discrete (Rep_of_Val v))\<close> and b16=None and TY16=\<open>typ_of_blk blk\<close>,
+            simplified])
+    apply blast
+    using \<F>_functional_condition_Rep_of_Val_ins_dom apply presburger
+    using prems apply blast
+    apply (rule rule1)
+    using prems apply blast
+    apply (rule refinement_projections_stepwise_UNIV_paired)
+    prefer 2
+    apply (rule rule1)
+    apply (simp add: prems)
+    apply (rule Rep_of_Val_ins.\<F>_functional_projection
+      [where S=\<open>{Some (discrete (Rep_of_Val v))}\<close> and TY=\<open>typ_of_blk blk\<close>, simplified])
+    using prems by blast
+qed .
+
+end
+
+end
+
+
+
+interpretation MovI: MoV id by (standard, simp)
+
 end
